Infra/LengthEq.v
@@ -37,6 +37,14 @@ Proof.
   intros H; general induction L; destruct L'; inv H; simpl; eauto.
 Qed.
 
+Lemma length_eq_dec {X} (L L' : list X)
+  : length_eq L L' + (length_eq L L' -> False).
+Proof.
+  destruct_prop(length L = length L').
+  left. eapply length_length_eq; eauto.
+  right. intro. eapply length_eq_length in X0. congruence.
+Defined.
+
 (* 
 *** Local Variables: ***
 *** coq-load-path: (("../" "Lvc")) ***
