LivenessValidators.v
@@ -1,0 +1,78 @@
+Require Import DecSolve IL Liveness LengthEq.
+
+Definition live_sound_dec Lv s slv (an:annotation s slv)
+      : Computable (live_sound Lv s slv).
+Proof. 
+  constructor.
+  general induction s; destruct slv; try isabsurd.
+  + edestruct IHs; eauto; try inv an; eauto;
+    destruct_prop (getAnn slv\{{x}} ⊆ a);
+    destruct_prop (live_exp_sound e a); try dec_solve.
+  + edestruct IHs1; try inv an; eauto;
+    edestruct IHs2; try inv an; eauto;
+    destruct_prop (x ∈ a); 
+    destruct_prop (getAnn slv1 ⊆ a); 
+    destruct_prop (getAnn slv2 ⊆ a);
+    try dec_solve; try eassumption; try inv an; eauto.
+  + destruct (get_dec Lv (counted l)) as [[[blv Z] ?]|?];
+    try destruct_prop ((blv \ of_list Z) ⊆ a);
+    destruct_prop (of_list Y ⊆ a);
+    try destruct_prop (length Y = length Z); try dec_solve.
+  +  destruct_prop(x ∈ a); try dec_solve.
+  + edestruct IHs1; eauto; try inv an; eauto;
+    edestruct IHs2; eauto; try inv an; eauto;
+    destruct_prop ((of_list Z) ⊆ getAnn slv1); 
+    destruct_prop ((getAnn slv1 \ of_list Z) ⊆ a);
+    destruct_prop (getAnn slv2 ⊆ a); try dec_solve.
+    Grab Existential Variables. eassumption. eassumption.
+Defined.
+
+
+Instance live_sound_dec_inst Lv s slv `{Computable(annotation s slv)}
+: Computable (live_sound Lv s slv).
+Proof.
+  destruct H as [[]].
+  eapply live_sound_dec; eauto.
+  constructor. right; intro. eauto using live_sound_annotation.
+Defined.
+
+Definition true_live_sound_dec Lv s slv (an:annotation s slv)
+      : Computable (true_live_sound Lv s slv).
+Proof. 
+  constructor.
+  general induction s; destruct slv; try isabsurd.
+  + edestruct IHs; eauto; try inv an; eauto;
+    destruct_prop (getAnn slv\{{x}} ⊆ a);
+    destruct_prop (x ∈ getAnn slv -> live_exp_sound e a); 
+(*    destruct_prop (x ∉ getAnn slv -> a ⊆ getAnn slv\{{x}});*) try dec_solve. 
+  + edestruct IHs1; try inv an; eauto;
+    edestruct IHs2; try inv an; eauto;
+    destruct_prop (x ∈ a); 
+    destruct_prop (getAnn slv1 ⊆ a); 
+    destruct_prop (getAnn slv2 ⊆ a);
+    try dec_solve; try eassumption; try inv an; eauto.
+  + destruct (get_dec Lv (counted l)) as [[[blv Z] ?]|?];
+    try destruct_prop ((blv \ of_list Z) ⊆ a);
+    try destruct_prop (argsLive a blv Y Z); try dec_solve.
+    left. econstructor; eauto using argsLive_length.
+  + destruct_prop(x ∈ a); try dec_solve.
+  + edestruct IHs1; eauto; try inv an; eauto;
+    edestruct IHs2; eauto; try inv an; eauto;
+    destruct_prop ((getAnn slv1 \ of_list Z) ⊆ a);
+    destruct_prop (getAnn slv2 ⊆ a); try dec_solve.
+    Grab Existential Variables. eassumption. eassumption.
+Defined.
+
+Instance true_live_sound_dec_inst Lv s slv `{Computable(annotation s slv)}
+: Computable (true_live_sound Lv s slv).
+Proof.
+  destruct H as [[]].
+  eapply true_live_sound_dec; eauto.
+  constructor. right; intro. eauto using true_live_sound_annotation.
+Defined.
+
+(* 
+*** Local Variables: ***
+*** coq-load-path: (("." "Lvc")) ***
+*** End: ***
+*)
